lib/Coqlib.v
@@ -24,3 +24,45 @@ Proof.
   intros.
   induction H; auto.
 Qed.
+
+(* This one copy from RamifyCoq *)
+Lemma Forall_app_iff: forall {A : Type} (P : A -> Prop) (l1 l2 : list A), Forall P (l1 ++ l2) <-> Forall P l1 /\ Forall P l2.
+Proof.
+  intros; induction l1; intros.
+  + simpl.
+    assert (Forall P nil) by constructor; tauto.
+  + simpl; split; intros.
+    - inversion H; subst; split; try tauto.
+      constructor; auto; tauto.
+    - destruct H.
+      inversion H; subst.
+      constructor; auto; tauto.
+Qed.
+
+Inductive remove_rel {A: Type}: A -> list A -> list A -> Prop :=
+| remove_rel_nil: forall a, remove_rel a nil nil
+| remove_rel_cons_eq: forall a xs ys, remove_rel a xs ys -> remove_rel a (a :: xs) ys
+| remove_rel_cons_neq: forall a b xs ys, a <> b -> remove_rel a xs ys -> remove_rel a (b :: xs) (b :: ys).
+
+Lemma remove_rel_In: forall (A : Type) (l1 l2 : list A) (x : A), remove_rel x l1 l2 -> ~ In x l2.
+Proof.
+  intros.
+  induction H.
+  + intros [].
+  + auto.
+  + intros [|]; auto.
+Qed.
+
+Lemma remove_rel_exist: forall (A : Type) (l1 : list A) (x : A) (DEC: forall y, x = y \/ x <> y), exists l2, remove_rel x l1 l2.
+Proof.
+  intros.
+  induction l1.
+  + exists nil.
+    apply remove_rel_nil.
+  + destruct IHl1 as [l2 ?].
+    destruct (DEC a).
+    - exists l2; subst.
+      apply remove_rel_cons_eq; auto.
+    - exists (a :: l2); subst.
+      apply remove_rel_cons_neq; auto.
+Qed.
