HenkinCompleteness.v
@@ -1,0 +1,24 @@
+Require Import Logic.LogicBase.
+Require Import Logic.SyntacticReduction.
+
+Local Open Scope logic_base.
+
+Lemma truth_lemma_from_syntactic_reduction {L: Language} (R: SyntacticReduction L) {sR: NormalSyntacticReduction L R} (SM: Semantics L) (Gamma: ProofTheory L):
+  reduction_consistent_prooftheory R Gamma ->
+  reduction_consistent_semantics R SM ->
+  forall (canonical_model: model) (Phi: context),
+    (forall x, Phi x <-> Phi |-- x) ->
+    (forall x: expr, normal_form x -> (canonical_model |= x <-> Phi x)) ->
+    (forall x: expr, canonical_model |= x <-> Phi x).
+Proof.
+  intros.
+  destruct (reduce_to_norm x) as [y [? ?]].
+  specialize (H2 y H4).
+  destruct H as [_ ?];
+  specialize (H Phi Phi x y (context_reduce_refl _) H3).
+  specialize (H0 x y canonical_model H3).
+  pose proof H1 x.
+  pose proof H1 y.
+  tauto.
+Qed.
+
