PropositionalLogic/ClassicalPropositionalLogic.v
@@ -1,3 +1,5 @@
+Require Import Coq.Logic.Classical_Prop.
+Require Import Logic.lib.Coqlib.
 Require Import Logic.LogicBase.
 Require Import Logic.SyntacticReduction.
 Require Import Logic.PropositionalLogic.Syntax.
@@ -24,7 +26,7 @@ Class ClassicalPropositionalLogic (L: Language) {nL: NormalLanguage L} {pL: Prop
   true_provable: provable TT
 }.
 
-Lemma imp_refl: forall (L: Language) {nL: NormalLanguage L} {pL: PropositionalLanguage L} {Gamma: ProofTheory L} {cpGamma: ClassicalPropositionalLogic L Gamma} (x: expr), |-- x --> x.
+Lemma imp_refl: forall {L: Language} {nL: NormalLanguage L} {pL: PropositionalLanguage L} {Gamma: ProofTheory L} {cpGamma: ClassicalPropositionalLogic L Gamma} (x: expr), |-- x --> x.
 Proof.
   intros.
   pose proof axiom2 x (x --> x) x.
@@ -42,14 +44,228 @@ Proof.
   eapply modus_ponens; eauto.
 Qed.
 
+Lemma aux_classic_theorem00: forall {L: Language} {nL: NormalLanguage L} {pL: PropositionalLanguage L} {Gamma: ProofTheory L} {cpGamma: ClassicalPropositionalLogic L Gamma} (x y z: expr), |--  (y --> z) --> (x --> y) --> (x --> z).
+Proof.
+  intros.
+  pose proof axiom2 x y z.
+  pose proof add_imp_left _ (y --> z) H.
+  pose proof axiom1 (y --> z) x.
+  pose proof axiom2 (y --> z) (x --> y --> z) ((x --> y) --> (x --> z)).
+  pose proof modus_ponens _ _ H2 H0.
+  pose proof modus_ponens _ _ H3 H1.
+  auto.
+Qed.
+
+Lemma remove_iden_assum_from_imp: forall {L: Language} {nL: NormalLanguage L} {pL: PropositionalLanguage L} {Gamma: ProofTheory L} {cpGamma: ClassicalPropositionalLogic L Gamma} (x y z: expr), |-- x --> y -> |-- (z --> x) --> (z --> y).
+Proof.
+  intros.
+  pose proof aux_classic_theorem00 z x y.
+  pose proof modus_ponens _ _ H0 H.
+  auto.
+Qed.
+
 Lemma imp_trans: forall {L: Language} {nL: NormalLanguage L} {pL: PropositionalLanguage L} {Gamma: ProofTheory L} {cpGamma: ClassicalPropositionalLogic L Gamma} (x y z: expr), |-- x --> y -> |-- y --> z -> |-- x --> z.
 Proof.
   intros.
-  pose proof add_imp_left _ x H0.
-  pose proof axiom2 x y z.
-  pose proof modus_ponens _ _ H2 H1.
-  pose proof modus_ponens _ _ H3 H.
+  pose proof aux_classic_theorem00 x y z.
+  pose proof modus_ponens _ _ H1 H0.
+  pose proof modus_ponens _ _ H2 H.
   auto.
+Qed.
+
+Lemma aux_classic_theorem01: forall {L: Language} {nL: NormalLanguage L} {pL: PropositionalLanguage L} {Gamma: ProofTheory L} {cpGamma: ClassicalPropositionalLogic L Gamma} (x y z: expr), |--  (x --> z) --> (x --> y --> z).
+Proof.
+  intros.
+  apply remove_iden_assum_from_imp.
+  apply axiom1.
+Qed.
+
+Lemma aux_classic_theorem02: forall {L: Language} {nL: NormalLanguage L} {pL: PropositionalLanguage L} {Gamma: ProofTheory L} {cpGamma: ClassicalPropositionalLogic L Gamma} (x y: expr), |-- x --> (x --> y) --> y.
+Proof.
+  intros.
+  pose proof axiom2 (x --> y) x y.
+  pose proof imp_refl (x --> y).
+  pose proof modus_ponens _ _ H H0.
+  pose proof remove_iden_assum_from_imp _ _ x H1.
+  pose proof axiom1 x (x --> y).
+  pose proof modus_ponens _ _ H2 H3.
+  auto.
+Qed.
+
+Lemma aux_classic_theorem03: forall {L: Language} {nL: NormalLanguage L} {pL: PropositionalLanguage L} {Gamma: ProofTheory L} {cpGamma: ClassicalPropositionalLogic L Gamma} (x y z: expr), |--  y --> (x --> y --> z) --> (x --> z).
+Proof.
+  intros.
+  pose proof aux_classic_theorem00 x (y --> z) z.
+  pose proof aux_classic_theorem02 y z.
+  eapply imp_trans; eauto.
+Qed.
+
+Lemma aux_classic_theorem04: forall {L: Language} {nL: NormalLanguage L} {pL: PropositionalLanguage L} {Gamma: ProofTheory L} {cpGamma: ClassicalPropositionalLogic L Gamma} (x y: expr), |-- (x --> x --> y) --> x --> y.
+Proof.
+  intros.
+  pose proof axiom2 x (x --> y) y.
+  pose proof aux_classic_theorem02 x y.
+  pose proof modus_ponens _ _ H H0.
+  auto.
+Qed.
+
+Lemma imp_arg_switch: forall {L: Language} {nL: NormalLanguage L} {pL: PropositionalLanguage L} {Gamma: ProofTheory L} {cpGamma: ClassicalPropositionalLogic L Gamma} (x y z: expr), |-- (x --> y --> z) --> (y --> x --> z).
+Proof.
+  intros.
+  apply imp_trans with (y --> x --> y --> z).
+  + apply axiom1.
+  + pose proof axiom2 y (x --> y --> z) (x --> z).
+    eapply modus_ponens; eauto. clear H.
+    pose proof aux_classic_theorem00 x (y --> z) z.
+    eapply imp_trans; eauto.
+    apply aux_classic_theorem02.
+Qed.
+
+Lemma imp_trans_strong: forall {L: Language} {nL: NormalLanguage L} {pL: PropositionalLanguage L} {Gamma: ProofTheory L} {cpGamma: ClassicalPropositionalLogic L Gamma} (x y z: expr), |-- (x --> y) --> (y --> z) --> (x --> z).
+Proof.
+  intros.
+  pose proof imp_arg_switch (y --> z) (x --> y) (x --> z).
+  eapply modus_ponens; eauto. clear H.
+  apply aux_classic_theorem00.
+Qed.
+
+Lemma multi_imp_arg_switch: forall {L: Language} {nL: NormalLanguage L} {pL: PropositionalLanguage L} {Gamma: ProofTheory L} {cpGamma: ClassicalPropositionalLogic L Gamma} (xs: list expr) (x y: expr), |-- (x --> multi_imp xs (x --> y)) --> multi_imp xs (x --> y).
+Proof.
+  intros.
+  induction xs.
+  + simpl.
+    apply aux_classic_theorem04.
+  + simpl.
+    apply remove_iden_assum_from_imp with (z := a) in IHxs.
+    eapply imp_trans; [| eauto].
+    apply imp_arg_switch.
+Qed.
+
+Lemma multi_imp_remove_rel: forall {L: Language} {nL: NormalLanguage L} {pL: PropositionalLanguage L} {Gamma: ProofTheory L} {cpGamma: ClassicalPropositionalLogic L Gamma} (xs1 xs2: list expr) (x y: expr), remove_rel x xs1 xs2 -> |-- multi_imp xs1 y --> multi_imp xs2 (x --> y).
+Proof.
+  intros.
+  induction H.
+  + simpl.
+    apply axiom1.
+  + simpl.
+    apply imp_trans with (a --> multi_imp ys (a --> y)).
+    - apply remove_iden_assum_from_imp; auto.
+    - apply multi_imp_arg_switch.
+  + simpl.
+    apply remove_iden_assum_from_imp; auto.
+Qed.
+
+Lemma derive_assum: forall {L: Language} {nL: NormalLanguage L} {pL: PropositionalLanguage L} {Gamma: ProofTheory L} {nGamma: NormalProofTheory L Gamma} {cpGamma: ClassicalPropositionalLogic L Gamma} (Phi: context) (x: expr), Phi x -> Phi |-- x.
+Proof.
+  intros.
+  rewrite derivable_provable.
+  exists (x :: nil); split.
+  + constructor; auto.
+  + simpl.
+    apply imp_refl.
+Qed.
+
+Lemma remove_rel_result_belong: forall (A : Type) (l1 l2 : list A) (x : A), remove_rel x l1 l2 -> Forall (fun y => In y l1) l2.
+Proof.
+  intros.
+  induction H.
+  + auto.
+  + simpl.
+    revert IHremove_rel; apply Forall_impl.
+    intros; auto.
+  + constructor; simpl; auto.
+    revert IHremove_rel; apply Forall_impl.
+    intros; auto.
+Qed.
+
+Lemma impp_elim: forall {L: Language} {nL: NormalLanguage L} {pL: PropositionalLanguage L} {Gamma: ProofTheory L} {nGamma: NormalProofTheory L Gamma} {cpGamma: ClassicalPropositionalLogic L Gamma} (Phi: context) (x y: expr),
+  Union _ Phi (Singleton _ x) |-- y ->
+  Phi |-- x --> y.
+Proof.
+  intros.
+  rewrite derivable_provable in H |- *.
+  destruct H as [xs [? ?]].
+  pose proof remove_rel_exist _ xs x (fun x => Classical_Prop.classic _).
+  destruct H1 as [xs' ?].
+  exists xs'; split.
+  + pose proof remove_rel_result_belong _ _ _ _ H1.
+    pose proof remove_rel_In _ _ _ _ H1.
+    rewrite Forall_forall in H, H2 |- *.
+    intros x0 HH; specialize (H2 x0 HH).
+    specialize (H x0 H2).
+    destruct H; auto.
+    inversion H; subst; contradiction.
+  + pose proof multi_imp_remove_rel xs xs' x y H1.
+    eapply modus_ponens; eauto.
+Qed.
+
+Lemma add_multi_imp_left_head: forall {L: Language} {nL: NormalLanguage L} {pL: PropositionalLanguage L} {Gamma: ProofTheory L} {cpGamma: ClassicalPropositionalLogic L Gamma} xs1 xs2 y, |-- multi_imp xs2 y --> multi_imp (xs1 ++ xs2) y.
+Proof.
+  intros.
+  induction xs1.
+  + apply imp_refl.
+  + eapply imp_trans; eauto.
+    apply axiom1.
+Qed.
+
+Lemma add_multi_imp_left_tail: forall {L: Language} {nL: NormalLanguage L} {pL: PropositionalLanguage L} {Gamma: ProofTheory L} {cpGamma: ClassicalPropositionalLogic L Gamma} xs1 xs2 y, |-- multi_imp xs1 y --> multi_imp (xs1 ++ xs2) y.
+Proof.
+  intros.
+  induction xs1; simpl.
+  + pose proof (add_multi_imp_left_head xs2 nil y).
+    rewrite app_nil_r in H; auto.
+  + apply remove_iden_assum_from_imp; auto.
+Qed.
+
+Lemma multi_imp_modus_ponens: forall {L: Language} {nL: NormalLanguage L} {pL: PropositionalLanguage L} {Gamma: ProofTheory L} {cpGamma: ClassicalPropositionalLogic L Gamma} xs y z, |-- multi_imp xs y --> multi_imp xs (y --> z) --> multi_imp xs z.
+Proof.
+  intros.
+  induction xs; simpl.
+  + apply aux_classic_theorem02.
+  + eapply imp_trans; [| apply imp_arg_switch].
+    eapply imp_trans; [| apply aux_classic_theorem04].
+    apply remove_iden_assum_from_imp.
+    eapply imp_trans; [eauto |].
+    eapply imp_trans; [| apply imp_arg_switch].
+    apply aux_classic_theorem00.
+Qed.
+
+Lemma derivable_modus_ponens: forall {L: Language} {nL: NormalLanguage L} {pL: PropositionalLanguage L} {Gamma: ProofTheory L} {nGamma: NormalProofTheory L Gamma} {cpGamma: ClassicalPropositionalLogic L Gamma} (Phi: context) (x y: expr),
+  Phi |-- x ->
+  Phi |-- x --> y ->
+  Phi |-- y.
+Proof.
+  intros.
+  rewrite derivable_provable in H, H0 |- *.
+  destruct H as [xs1 [? ?]], H0 as [xs2 [? ?]].
+  exists (xs1 ++ xs2); split.
+  + rewrite Forall_app_iff; auto.
+  + pose proof modus_ponens _ _ (add_multi_imp_left_tail xs1 xs2 _) H1.
+    pose proof modus_ponens _ _ (add_multi_imp_left_head xs1 xs2 _) H2.
+    pose proof multi_imp_modus_ponens (xs1 ++ xs2) x y.
+    pose proof modus_ponens _ _ H5 H3.
+    pose proof modus_ponens _ _ H6 H4.
+    auto.
+Qed.
+
+Lemma MCS_element_derivable: forall {L: Language} {nL: NormalLanguage L} {pL: PropositionalLanguage L} {Gamma: ProofTheory L} {nGamma: NormalProofTheory L Gamma} {cpGamma: ClassicalPropositionalLogic L Gamma} (Phi: context),
+  maximal_consistent Gamma Phi ->
+  (forall x: expr, Phi x <-> Phi |-- x).
+Proof.
+  intros.
+  split; [apply derive_assum | intros].
+  assert (consistent Gamma (Union _ Phi (Singleton _ x))).
+  Focus 1. {
+    intro.
+    pose proof impp_elim _ _ _ H1.
+    pose proof derivable_modus_ponens _ _ _ H0 H2.
+    destruct H; auto.
+  } Unfocus.
+  destruct H.
+  specialize (H2 _ H1).
+  specialize (H2 (fun x H => Union_introl _ _ _ x H)).
+  apply H2.
+  right; constructor.
 Qed.
 
 Module ClassicalPropositionalLogic.
