PropositionalLogic/Complete_Classical_Trivial.v
@@ -1,4 +1,6 @@
 Require Import Logic.LogicBase.
+Require Import Logic.SyntacticReduction.
+Require Import Logic.HenkinCompleteness.
 Require Import Logic.PropositionalLogic.Syntax.
 Require Import Logic.PropositionalLogic.ClassicalPropositionalLogic.
 Require Import Logic.PropositionalLogic.TrivialSemantics.
@@ -14,4 +16,8 @@ Definition canonical_model {Var: Type} (Phi: MCS Var): @model _ (TrivialSemantic
 Lemma truth_lemma {Var: Type}: forall (Phi: MCS Var) x, canonical_model Phi |= x <-> proj1_sig Phi x.
 Proof.
   intros.
+  revert x.
+  pose proof @MCS_element_derivable _ _ _ _ _ (ClassicalPropositionalLogic.cpG Var) (proj1_sig Phi) (proj2_sig Phi).
+  pose proof @TrivialSemantics.mendelson_consistent Var.
+  apply (@truth_lemma_from_syntactic_reduction _ (PropositionalLanguage.MendelsonReduction Var) (PropositionalLanguage.nMendelsonReduction) _ (ClassicalPropositionalLogic.G Var)).
 Abort.
