PropositionalLogic/Sound_Classical_Trivial.v
@@ -7,108 +7,6 @@ Require Import Logic.PropositionalLogic.TrivialSemantics.
 Local Open Scope logic_base.
 Local Open Scope PropositionalLogic.
 
-Lemma sound_ImpNegAsPrime {Var: Type}:
-  forall x y: @expr (PropositionalLanguage.L Var),
-    ImpNegAsPrime.atomic_reduce x y ->
-    forall m: @model _ (TrivialSemantics.SM Var), m |= x <-> m |= y.
-Proof.
-  intros; split; intros; destruct H; auto.
-Qed.
-
-Lemma sound_ReduceIff {Var: Type}:
-  forall x y: @expr (PropositionalLanguage.L Var),
-    ReduceIff.atomic_reduce x y ->
-    forall m: @model _ (TrivialSemantics.SM Var), m |= x <-> m |= y.
-Proof.
-  intros; split; intros; destruct H; auto.
-Qed.
-
-Lemma sound_ReduceFalse {Var: Type}:
-  forall x y: @expr (PropositionalLanguage.L Var),
-    ReduceFalse.atomic_reduce x y ->
-    forall m: @model _ (TrivialSemantics.SM Var), m |= x <-> m |= y.
-Proof.
-  intros; split; intros; destruct H.
-  + simpl in H0.
-    inversion H0.
-  + specialize (H0 I).
-    inversion H0.
-Qed.
-
-Lemma sound_disjunction {Var: Type}:
-  forall reduce1 reduce2: relation (@expr (PropositionalLanguage.L Var)),
-    (forall x y, reduce1 x y -> forall m: @model _ (TrivialSemantics.SM Var), m |= x <-> m |= y) ->
-    (forall x y, reduce2 x y -> forall m: @model _ (TrivialSemantics.SM Var), m |= x <-> m |= y) ->
-    (forall x y, relation_disjunction reduce1 reduce2 x y -> forall m: @model _ (TrivialSemantics.SM Var), m |= x <-> m |= y).
-Proof.
-  intros.
-  destruct H1.
-  + apply H; auto.
-  + apply H0; auto.
-Qed.
-
-Lemma sound_propag_reduce {Var: Type}:
-  forall reduce: relation (@expr (PropositionalLanguage.L Var)),
-    (forall x y, reduce x y -> forall m: @model _ (TrivialSemantics.SM Var), m |= x <-> m |= y) ->
-    (forall x y, propag_reduce reduce x y -> forall m: @model _ (TrivialSemantics.SM Var), m |= x <-> m |= y).
-Proof.
-  intros.
-  destruct H0.
-  induction p as [| [| | | | | | | |]].
-  + simpl; apply H; auto.
-  + simpl in *.
-    unfold TrivialSemantics.sem_and, TrivialSemantics.sem_neg, TrivialSemantics.sem_imp; simpl.
-    tauto.
-  + simpl in *.
-    unfold TrivialSemantics.sem_and, TrivialSemantics.sem_neg, TrivialSemantics.sem_imp; simpl.
-    tauto.
-  + simpl in *.
-    unfold TrivialSemantics.sem_or, TrivialSemantics.sem_neg, TrivialSemantics.sem_imp; simpl.
-    tauto.
-  + simpl in *.
-    unfold TrivialSemantics.sem_or, TrivialSemantics.sem_neg, TrivialSemantics.sem_imp; simpl.
-    tauto.
-  + simpl in *.
-    unfold TrivialSemantics.sem_imp; simpl.
-    tauto.
-  + simpl in *.
-    unfold TrivialSemantics.sem_imp; simpl.
-    tauto.
-  + simpl in *.
-    unfold TrivialSemantics.sem_iff, TrivialSemantics.sem_and, TrivialSemantics.sem_neg, TrivialSemantics.sem_imp; simpl.
-    tauto.
-  + simpl in *.
-    unfold TrivialSemantics.sem_iff, TrivialSemantics.sem_and, TrivialSemantics.sem_neg, TrivialSemantics.sem_imp; simpl.
-    tauto.
-  + simpl in *.
-    unfold TrivialSemantics.sem_neg; simpl.
-    tauto.
-Qed.
-
-Lemma sound_clos_refl_trans {Var: Type}:
-  forall reduce: relation (@expr (PropositionalLanguage.L Var)),
-    (forall x y, reduce x y -> forall m: @model _ (TrivialSemantics.SM Var), m |= x <-> m |= y) ->
-    (forall x y, clos_refl_trans expr reduce x y -> forall m: @model _ (TrivialSemantics.SM Var), m |= x <-> m |= y).
-Proof.
-  intros.
-  induction H0.
-  + apply H; auto.
-  + tauto.
-  + tauto.
-Qed.
-
-Lemma sound_reduce {Var: Type}:
-  forall x y: @expr (PropositionalLanguage.L Var), reduce x y ->
-    forall m: @model _ (TrivialSemantics.SM Var), m |= x <-> m |= y.
-Proof.
-  apply sound_clos_refl_trans.
-  apply sound_propag_reduce.
-  repeat apply sound_disjunction.
-  + apply sound_ImpNegAsPrime.
-  + apply sound_ReduceIff.
-  + apply sound_ReduceFalse.
-Qed.
-
 Lemma sound_modus_ponens {Var: Type}:
   forall x y: @expr (PropositionalLanguage.L Var),
     forall m: @model _ (TrivialSemantics.SM Var),
@@ -157,10 +55,8 @@ Proof.
   hnf; intros.
   intro m.
   induction H.
-  + pose proof sound_reduce x y H.
-    exact (proj1 (H1 m) IHprovable).
-  + pose proof sound_reduce x y H.
-    exact (proj2 (H1 m) IHprovable).
+  + rewrite <- (TrivialSemantics.mendelson_consistent x y m H); auto.
+  + rewrite -> (TrivialSemantics.mendelson_consistent x y m H); auto.
   + pose proof sound_modus_ponens x y.
     exact (H1 m IHprovable1 IHprovable2).
   + apply sound_axiom1.
