PropositionalLogic/TrivialSemantics.v
@@ -1,4 +1,5 @@
 Require Import Logic.LogicBase.
+Require Import Logic.SyntacticReduction.
 Require Import Logic.PropositionalLogic.Syntax.
 Require Import Coq.Logic.Classical_Prop.
 
@@ -38,4 +39,97 @@ Fixpoint denotation {Var: Type} (x: expr Var): Ensemble (model Var) :=
 Instance SM (Var: Type): Semantics (PropositionalLanguage.L Var) :=
   Build_Semantics (PropositionalLanguage.L Var) (model Var) (fun m x => denotation x m).
 
+Local Open Scope logic_base.
+Local Open Scope PropositionalLogic.
+
+Lemma ImpNegAsPrime_consistent {Var: Type}:
+  forall x y: expr Var,
+    @ImpNegAsPrime.atomic_reduce (L Var) (nL Var) (pL Var) x y ->
+    forall m: model Var, denotation x m <-> denotation y m.
+Proof.
+  intros; split; intros; destruct H; auto.
+Qed.
+
+Lemma ReduceIff_consistent {Var: Type}:
+  forall x y: expr Var,
+    @ReduceIff.atomic_reduce (L Var) (nL Var) (pL Var) x y ->
+    forall m: model Var, denotation x m <-> denotation y m.
+Proof.
+  intros; split; intros; destruct H; auto.
+Qed.
+
+Lemma ReduceFalse_consistent {Var: Type}:
+  forall x y: expr Var,
+    @ReduceFalse.atomic_reduce (L Var) (nL Var) (pL Var) x y ->
+    forall m: model Var, denotation x m <-> denotation y m.
+Proof.
+  intros; split; intros; destruct H.
+  + simpl in H0.
+    inversion H0.
+  + specialize (H0 I).
+    inversion H0.
+Qed.
+
+Lemma disjunction_reduce_consistent {Var: Type}:
+  forall reduce1 reduce2: relation (expr Var),
+    (forall x y, reduce1 x y -> forall m: model Var, denotation x m <-> denotation y m) ->
+    (forall x y, reduce2 x y -> forall m: model Var, denotation x m <-> denotation y m) ->
+    forall x y, relation_disjunction reduce1 reduce2 x y ->
+    forall m: model Var, denotation x m <-> denotation y m.
+Proof.
+  intros.
+  destruct H1.
+  + apply H; auto.
+  + apply H0; auto.
+Qed.
+
+Lemma propag_reduce_consistent {Var: Type}:
+  forall reduce: relation (expr Var),
+    (forall x y, reduce x y -> forall m: model Var, denotation x m <-> denotation y m) ->
+    (forall x y, @propag_reduce (L Var) reduce x y -> forall m: model Var, denotation x m <-> denotation y m).
+Proof.
+  intros.
+  destruct H0.
+  induction p as [| [| | | | | | | |]].
+  + simpl; apply H; auto.
+  + simpl in *.
+    unfold TrivialSemantics.sem_and, TrivialSemantics.sem_neg, TrivialSemantics.sem_imp; simpl.
+    tauto.
+  + simpl in *.
+    unfold TrivialSemantics.sem_and, TrivialSemantics.sem_neg, TrivialSemantics.sem_imp; simpl.
+    tauto.
+  + simpl in *.
+    unfold TrivialSemantics.sem_or, TrivialSemantics.sem_neg, TrivialSemantics.sem_imp; simpl.
+    tauto.
+  + simpl in *.
+    unfold TrivialSemantics.sem_or, TrivialSemantics.sem_neg, TrivialSemantics.sem_imp; simpl.
+    tauto.
+  + simpl in *.
+    unfold TrivialSemantics.sem_imp; simpl.
+    tauto.
+  + simpl in *.
+    unfold TrivialSemantics.sem_imp; simpl.
+    tauto.
+  + simpl in *.
+    unfold TrivialSemantics.sem_iff, TrivialSemantics.sem_and, TrivialSemantics.sem_neg, TrivialSemantics.sem_imp; simpl.
+    tauto.
+  + simpl in *.
+    unfold TrivialSemantics.sem_iff, TrivialSemantics.sem_and, TrivialSemantics.sem_neg, TrivialSemantics.sem_imp; simpl.
+    tauto.
+  + simpl in *.
+    unfold TrivialSemantics.sem_neg; simpl.
+    tauto.
+Qed.
+
+Lemma mendelson_consistent {Var: Type}: reduction_consistent_semantics (MendelsonReduction Var) (SM Var).
+Proof.
+  apply reduction_consistent_semantics_spec.
+  apply propag_reduce_consistent.
+  repeat apply disjunction_reduce_consistent.
+  + apply ImpNegAsPrime_consistent.
+  + apply ReduceIff_consistent.
+  + apply ReduceFalse_consistent.
+Qed.
+
 End TrivialSemantics.
+
